prelude/base.v
@@ -30,7 +30,7 @@ Ltac properness :=
   | |- (WP _ {{ _ }})%I ≡ (WP _ {{ _ }})%I => apply wp_proper =>?
   | |- (▷ _)%I ≡ (▷ _)%I => apply later_proper
   | |- (□ _)%I ≡ (□ _)%I => apply always_proper
-  | |- (_ ★ _)%I ≡ (_ ★ _)%I => apply sep_proper
+  | |- (_ ∗ _)%I ≡ (_ ∗ _)%I => apply sep_proper
   | |- (inv _ _)%I ≡ (inv _ _)%I => apply (contractive_proper _)
   end.
 
